---
title: "memo-KPR"
format: html
---

Proposition:

For the utility function
$$
U = \frac{1}{1-\gamma-\xi}\left[ C^{1-\gamma} - \frac{1-\gamma}{1+\varphi} N^{1+\varphi} \right]^{1 - \xi/(1-\gamma)},
$$
as $\gamma \to 1$, the limit is:
$$
U \to -\frac{1}{\xi}\left[ C \exp\left( -\frac{1}{1+\varphi} N^{1+\varphi} \right) \right]^{-\xi}.
$$
---

**Proof:**

Let $\varepsilon = 1 - \gamma$ and consider the limit $\varepsilon \to 0$.

---

### 1. Expansion of the inner term

$$
C^{1-\gamma} = C^{\varepsilon} = e^{\varepsilon \ln C} = 1 + \varepsilon \ln C + O(\varepsilon^2).
$$
$$
\frac{1-\gamma}{1+\varphi} N^{1+\varphi} = \frac{\varepsilon}{1+\varphi} N^{1+\varphi}.
$$

Therefore,
$$
A \equiv C^{\varepsilon} - \frac{\varepsilon}{1+\varphi} N^{1+\varphi}
= 1 + \varepsilon \left( \ln C - \frac{N^{1+\varphi}}{1+\varphi} \right) + O(\varepsilon^2).
$$

---

### 2. Taking logs

$$
\ln A = \varepsilon B + O(\varepsilon^2), \quad 
B = \ln C - \frac{N^{1+\varphi}}{1+\varphi}.
$$

---

### 3. Log of the power term

Since the outer exponent is $1 - \frac{\xi}{\varepsilon}$,

$$
\ln \left(A^{1 - \frac{\xi}{\varepsilon}}\right) = \left(1 - \frac{\xi}{\varepsilon} \right) \ln A
= \left(1 - \frac{\xi}{\varepsilon} \right) \left[ \varepsilon B + O(\varepsilon^2) \right]
$$

$$
= \varepsilon B - \xi B + O(\varepsilon).
$$

As $\varepsilon \to 0$, the $O(\varepsilon)$ term vanishes, and

$$
\ln \left(A^{1 - \frac{\xi}{\varepsilon}}\right) \to -\xi B.
$$

---

### 4. Exponentiating the power term

$$
\begin{aligned}
A^{1 - \frac{\xi}{\varepsilon}} &\to e^{-\xi B} 
= e^{-\xi \left( \ln C - \frac{N^{1+\varphi}}{1+\varphi} \right)}\\
&= C^{-\xi} \cdot \exp\left( \frac{\xi}{1+\varphi} N^{1+\varphi} \right).
\end{aligned}
$$

The prefactor satisfies
$$
\frac{1}{1-\gamma-\xi} = \frac{1}{\varepsilon - \xi} \to -\frac{1}{\xi}.
$$

---

### 5. Alternative expression of the result

On the other hand, the target expression
$$
-\frac{1}{\xi}\left[ C \exp\left( -\frac{1}{1+\varphi} N^{1+\varphi} \right) \right]^{-\xi}
$$
is
$$
= -\frac{1}{\xi} C^{-\xi} \cdot \exp\left( -\xi \cdot \left[ -\frac{N^{1+\varphi}}{1+\varphi} \right] \right)
= -\frac{1}{\xi} C^{-\xi} \cdot \exp\left( \frac{\xi}{1+\varphi} N^{1+\varphi} \right).
$$
which matches the limit obtained above exactly.

---

Therefore, as $\gamma \to 1$,
$$
\frac{1}{1-\gamma-\xi}\left[ C^{1-\gamma} - \frac{1-\gamma}{1+\varphi} N^{1+\varphi} \right]^{1 - \xi/(1-\gamma)}
\longrightarrow
-\frac{1}{\xi}\left[ C \exp\left( -\frac{1}{1+\varphi} N^{1+\varphi} \right) \right]^{-\xi}
$$
is established.

QED.
