%% LyX 2.4.4 created this file.  For more info, see https://www.lyx.org/.
%% Do not edit unless you really know what you are doing.
\documentclass[english,autodetect-engine, dvi=dvipdfmx, ja=standard]{bxjsarticle}
\usepackage[T1]{fontenc}
\usepackage[utf8]{luainputenc}
\usepackage{varwidth}
\usepackage{amsmath}
\usepackage{amssymb}

\makeatletter

%%%%%%%%%%%%%%%%%%%%%%%%%%%%%% LyX specific LaTeX commands.
%% Because html converters don't know tabularnewline
\providecommand{\tabularnewline}{\\}
%% Variable width box for table cells
\newenvironment{cellvarwidth}[1][t]
    {\begin{varwidth}[#1]{\linewidth}}
    {\@finalstrut\@arstrutbox\end{varwidth}}

\makeatother

\usepackage{babel}
\begin{document}
Variables:

\begin{tabular}{|c|c|}
\hline 
 & description\tabularnewline
\hline 
\hline 
$C$ & Consumption\tabularnewline
\hline 
$C^{S}$ & Consumption, S\tabularnewline
\hline 
$C^{H}$ & Consumption, H\tabularnewline
\hline 
$N$ & Labor Inputs\tabularnewline
\hline 
$N^{S}$ & Labor Inputs, S\tabularnewline
\hline 
$N^{H}$ & Labor Inputs, H\tabularnewline
\hline 
$Y$ & Output\tabularnewline
\hline 
$W$ & Wage Rate\tabularnewline
\hline 
$D$ & Dividends\tabularnewline
\hline 
$\Pi$ & Rates of Inflation\tabularnewline
\hline 
$R^{N}$ & Nominal Rates of Interests\tabularnewline
\hline 
$R$ & Real Rates of Interests\tabularnewline
\hline 
$MC$ & Marginal Cost\tabularnewline
\hline 
$MU$ & Marginal Utility\tabularnewline
\hline 
$m_{t}$ & Monetary shock\tabularnewline
\hline 
\end{tabular}

Parameters

\begin{tabular}{|c|c|}
\hline 
 & \tabularnewline
\hline 
\hline 
$\gamma$ & income effect\tabularnewline
\hline 
$\varphi$ & inverse of wage elasticity wrt labor inputs\tabularnewline
\hline 
$\xi$ & degree of non-separability\tabularnewline
\hline 
$\kappa^{S}$ & \begin{cellvarwidth}[t]
\centering
degree of complementarity\\
$\kappa^{S}=\left[1-\frac{(1-\gamma)(1-\alpha)(1-\Phi)}{1+\varphi}\frac{N^{S}/N}{C^{S}/Y}\right]^{-1}\xi$
\end{cellvarwidth}\tabularnewline
\hline 
$\psi$ & Elasticity of substitution between intermediate inputs\tabularnewline
\hline 
$\eta$ & price adjustment cost\tabularnewline
\hline 
$\tau$ & tax rate on dividends\tabularnewline
\hline 
$\sigma$ & subsidy rate on intermediate goods\tabularnewline
\hline 
$\Phi$ & degree of efficiency $\Phi=(1-1/\psi)(1+\sigma)-1$\tabularnewline
\hline 
$\lambda$ & ratio of type H consumers\tabularnewline
\hline 
$\beta$ & discount rate\tabularnewline
\hline 
$\alpha$ & capital share\tabularnewline
\hline 
$\phi$ & Taylor rule parameter\tabularnewline
\hline 
$\rho$ & persistency of monetary shock\tabularnewline
\hline 
\end{tabular}

Equation:
\begin{center}
\begin{tabular}{l|c}
\hline 
Name & Equation\tabularnewline
\hline 
Euler equation, S & $r_{t}=mu_{t}^{S}-E_{t}mu_{t+1}^{S}$\tabularnewline
Marginal utility, S & $mu_{t}^{S}=-(\gamma+\kappa^{S})c_{t}^{S}+\kappa^{S}(1-\alpha)(1-\Phi)\frac{N^{S}/N}{C^{S}/Y}n_{t}^{S}$\tabularnewline
Labor supply, S & $w_{t}=\gamma c_{t}^{S}+\varphi n_{t}^{S}$\tabularnewline
Labor supply, H & $w_{t}=\gamma c_{t}^{H}+\varphi n_{t}^{H}$\tabularnewline
Budget constraint, H & $\frac{C^{H}}{Y}c_{t}^{H}=\frac{WN^{H}}{Y}(w_{t}+n_{t}^{H})+\frac{\tau^{D}}{\lambda}d_{t}$\tabularnewline
Labor demand & $w_{t}=mc_{t}+y_{t}-n_{t}$\tabularnewline
Phillips curve & $\pi_{t}=(\psi_{p}/\eta_{p})(1-\Phi)mc_{t}+\beta E_{t}\pi_{t+1}$\tabularnewline
Profits & $d_{t}=\Phi y_{t}-(1-\alpha)(1-\Phi)w_{t}$\tabularnewline
Aggregate consumption & $c_{t}=\lambda\frac{C^{H}}{C}c_{t}^{H}+(1-\lambda)\frac{C^{S}}{C}c_{t}^{S}$\tabularnewline
Aggregate labor & $n_{t}=\lambda\frac{N^{H}}{N}n_{t}^{H}+(1-\lambda)\frac{N^{S}}{N}n_{t}^{S}$\tabularnewline
Production function & $y_{t}=(1-\alpha)n_{t}$\tabularnewline
Resource constraint & $y_{t}=c_{t}$\tabularnewline
Taylor rule & $r_{t}^{N}=\phi\pi_{t}^{p}-m_{t}$\tabularnewline
Monetary shock & $m_{t}=\rho m_{t-1}+e_{t}$\tabularnewline
Fischer equation & $r_{t}=r_{t}^{N}-E_{t}\pi_{t+1}$\tabularnewline
\hline 
\end{tabular}
\par\end{center}
\begin{itemize}
\item 15変数 ($D_{t},W_{t},N_{t},N_{t}^{H},N_{t}^{S},MC_{t},C_{t},C_{t}^{H},C_{t}^{S},Y_{t},R_{t}^{N}$,
$\Pi_{t}$,$MU_{t}^{S}$,$MC_{t}$, $m_{t}$):
\begin{align*}
W_{t} & =\Xi(N_{t}^{H})^{\varphi}(C_{t}^{H})^{\gamma}\\
C_{t}^{H} & =W_{t}N_{t}^{H}+\frac{\tau^{D}}{\lambda}D_{t}\\
W_{t} & =\Xi(N_{t}^{S})^{\varphi}(C_{t}^{S})^{\gamma}\\
1 & =\mathbb{E}_{t}\left[\beta R_{t}\frac{MU_{t+1}^{S}}{MU_{t}^{S}}\right]\\
R_{t} & =\mathbb{E}_{t}\left[\frac{R_{t}^{N}}{\Pi_{t+1}}\right]\\
MU_{t}^{S} & =(C_{t}^{S})^{-\gamma}\left(\frac{(C_{t}^{S})^{1-\gamma}}{1-\gamma}-\chi\frac{(N_{t}^{S})^{1+\varphi}}{1+\varphi}\right)^{-\xi/(1-\gamma)}
\end{align*}
\begin{align*}
W_{t} & =(1-\alpha)MC_{t}N_{t}^{-\alpha}\\
D_{t}= & Y_{t}-\frac{\eta_{P}}{2}\left(\frac{\Pi_{t}}{\Pi}-1\right)^{2}Y_{t}-W_{t}N_{t}
\end{align*}
\begin{align*}
\eta_{P}\frac{\Pi_{t}}{\Pi}\left(\frac{\Pi_{t}}{\Pi}-1\right)=\psi_{P}\left(MC_{t}-(1+\tau^{S})(1-1/\psi_{P})\right)\\
+\beta\eta_{P}\mathbb{E}_{t}\left[\left(\frac{C_{t+1}^{S}}{C_{t}^{S}}\right)^{-\sigma}\frac{Y_{t+1}}{Y_{t}}\frac{\Pi_{t+1}}{\Pi}\left(\frac{\Pi_{t+1}}{\Pi}-1\right)\right]
\end{align*}
\end{itemize}
\begin{align*}
C_{t} & =\lambda C_{t}^{H}+(1-\lambda)C_{t}^{S}\\
N_{t} & =\lambda N_{t}^{S}+(1-\lambda)N_{t}^{S}\\
Y_{t} & =C_{t}+\frac{\eta_{P}}{2}\left(\frac{\Pi_{t}}{\Pi}-1\right)^{2}Y_{t}\\
Y_{t} & =N_{t}^{1-\alpha}\\
\frac{R_{t}^{N}}{R^{N}} & =\left(\frac{\Pi_{t}}{\Pi}\right)^{\phi}\exp(-m_{t})\\
m_{t} & =\rho_{m}m_{t-1}+e_{t}^{m}
\end{align*}

\begin{itemize}
\item 定常状態
\begin{align*}
W & =\Xi(N^{H})^{\varphi}(C^{H})^{\gamma}\\
C^{H} & =WN^{H}+\frac{\tau^{D}}{\lambda}D\\
W & =\Xi(N^{S})^{\varphi}(C^{S})^{\gamma}\\
1 & =\mathbb{E}_{t}\left[\beta\frac{R^{N}}{\Pi}\right]\\
MU^{S} & =(C^{S})^{-\gamma}\left(\frac{(C^{S})^{1-\gamma}}{1-\gamma}-\chi\frac{(N^{S})^{1+\varphi}}{1+\varphi}\right)^{-\xi/(1-\gamma)}
\end{align*}
\begin{align*}
W & =(1-\alpha)MCN^{-\alpha}\\
D=Y & -WN
\end{align*}
\[
MC=(1+\sigma)(1-1/\psi)
\]
\end{itemize}
\begin{align*}
C & =\lambda C^{H}+(1-\lambda)C^{S}\\
N & =\lambda N^{H}+(1-\lambda)N^{S}\\
Y & =C\\
Y & =N^{1-\alpha}
\end{align*}

\begin{itemize}
\item 対数線形近は以下である $d_{t}=(D_{t}-D)/Y$:
\begin{align*}
w_{t} & =\varphi n_{t}^{H}+\gamma c_{t}^{H}\\
\frac{C^{H}}{Y}c_{t}^{H} & =\frac{WN^{H}}{Y}(w_{t}+n_{t}^{H})+\frac{\tau^{D}}{\lambda}d_{t}\\
w_{t} & =\varphi n_{t}^{S}+\gamma c_{t}^{S}\\
r_{t}^{N} & =\mathbb{E}_{t}\left[\pi_{t+1}\right]-\mathbb{E}_{t}\left[\Delta mu_{t+1}^{S}\right]
\end{align*}
\begin{align*}
mu_{t}^{S} & =-(\gamma+\kappa)c_{t}^{S}+\kappa^{S}(1-\alpha)MC\frac{N^{S}/N}{C^{S}/Y}n_{t}^{S}\\
\kappa^{S} & =\xi\left[1-\frac{1-\gamma}{1+\varphi}(1-\alpha)MC\frac{N^{S}/N}{C^{S}/Y}\right]^{-1}
\end{align*}
\begin{align*}
w_{t}= & mc_{t}+y_{t}-n_{t}\\
d_{t}= & (1-MC)y_{t}-(1-\alpha)MCw_{t}\\
\pi_{t}= & \frac{\psi_{p}MC}{\eta_{p}}mc_{t}+\beta\mathbb{E}_{t}\left[\pi_{t+1}\right]
\end{align*}
\begin{align*}
c_{t} & =\lambda\frac{C^{H}}{C}c_{t}^{H}+(1-\lambda)\frac{C^{S}}{C}c_{t}^{S}\\
n_{t} & =\lambda\frac{N^{H}}{N}n_{t}^{H}+(1-\lambda)\frac{N^{S}}{N}n_{t}^{S}\\
y_{t} & =c_{t}\\
y_{t} & =(1-\alpha)n_{t}\\
r_{t}^{N} & =\phi\pi_{t}-m_{t}\\
m_{t} & =\rho_{m}m_{t-1}+e_{t}^{m}
\end{align*}
\item If $\Xi=1$, $\Pi=1$, $MC=1$, $\alpha=0$, then $C=C^{S}=C^{H}=N=N^{S}=N^{H}=Y=W=1$,
$D=0$, $R^{N}=1/\beta$.
\begin{align*}
w_{t} & =\varphi n_{t}^{H}+\gamma c_{t}^{H}\\
c_{t}^{H} & =w_{t}+n_{t}^{H}+\frac{\tau^{D}}{\lambda}d_{t}\\
w_{t} & =\varphi n_{t}^{S}+\gamma c_{t}^{S}\\
r_{t}^{N} & =\mathbb{E}_{t}\left[\pi_{t+1}\right]-\mathbb{E}_{t}\left[\Delta mu_{t+1}^{S}\right]
\end{align*}
\begin{align*}
mu_{t}^{S} & =-(\gamma+\kappa^{S})c_{t}^{S}+\kappa^{S}n_{t}^{S}\\
\kappa^{S} & =\xi\left[1-\frac{1-\gamma}{1+\varphi}\right]^{-1}=\frac{\varphi+\gamma}{1+\varphi}\xi
\end{align*}
\begin{align*}
w_{t}= & mc_{t}\\
d_{t}= & -w_{t}\\
\pi_{t}= & \frac{\psi_{p}(\varphi+\gamma)}{\eta_{p}}mc_{t}+\beta\mathbb{E}_{t}\left[\pi_{t+1}\right]
\end{align*}
\end{itemize}
\begin{align*}
c_{t} & =\lambda c_{t}^{H}+(1-\lambda)c_{t}^{S}\\
n_{t} & =\lambda n_{t}^{H}+(1-\lambda)n_{t}^{S}\\
y_{t} & =c_{t}\\
y_{t} & =(1-\alpha)n_{t}\\
r_{t}^{N} & =\phi\pi_{t}-m_{t}\\
m_{t} & =\rho_{m}m_{t-1}+e_{t}^{m}
\end{align*}

General solution:
\begin{align*}
c_{t}^{H} & =(1+\tilde{\tilde{\varphi}})y_{t}\\
c_{t}^{S} & =\left\{ 1-\frac{\lambda\tilde{\tilde{\varphi}}}{1-\lambda}\right\} y_{t}\\
n_{t}^{H} & =(1-\tilde{\tilde{\gamma}})y_{t}\\
n_{t}^{S} & =\left\{ \frac{1-\lambda(1-\alpha)}{(1-\alpha)(1-\lambda)}+\frac{\lambda\tilde{\tilde{\gamma}}}{1-\lambda}\right\} y_{t}\\
w_{t} & =(\gamma+\varphi)(1+\tilde{\alpha})y_{t}=\frac{(1-\alpha)\gamma+\varphi}{(1-\alpha)}y_{t}\\
d_{t} & =\Phi y_{t}-(1-\alpha)(1-\Phi)w_{t}\\
 & =\{\Phi-(1-\Phi)\{(1-\alpha)\gamma+\varphi\}\}y_{t}\\
mc_{t} & =w_{t}+y_{t}\alpha/(1-\alpha)=\left\{ \gamma+\frac{\varphi+\alpha}{1-\alpha}\right\} y_{t}\\
\pi_{t} & =\frac{\psi_{p}(1-\Phi)}{\eta_{p}}mc_{t}+\beta\mathbb{E}_{t}\left[\pi_{t+1}\right]\\
r_{t}^{N} & =\phi\pi_{t}-m_{t}\\
mu_{t}^{S} & =-(\gamma+\kappa^{S})c_{t}^{S}+\kappa^{S}n_{t}^{S}\\
r_{t} & =mu_{t}^{S}-E_{t}mu_{t+1}^{S}\\
r_{t} & =r_{t}^{N}-E_{t}\pi_{t+1}
\end{align*}

\end{document}
